\documentclass[a4paper,12pt]{article}

\usepackage{worksheet}

\newcommand{\deriv}[3][]{\frac{d^{#1}#2}{d#3^{#1}}}

\begin{document}

\section*{Finding Derivatives Starter}

\subsection*{Question Bank}

\begin{enumerate}
\item For each of the following functions, find their derivatives by first 
principles. %Recall that the first principles formula is,
%$f'(x) = \lim_{h\to 0}\frac{f(x + h) - f(x)}{h}$.
\begin{multicols}{2}
    \begin{enumerate}
    \item \sspacer$f(x) = x^3$
    \item \sspacer$f(x) = 4x$
    \item \sspacer$f(x) = 2x^2 - 3x$
    \item \sspacer$f(x) = x(2x + 1)$
    \item \sspacer$f(x) = (x^2 + 2)(x - 4)$
    \item \sspacer$f(x) = \frac{x + 2}{x}$
    \end{enumerate}
    \end{multicols}

\item For each of the following functions, find their derivatives by applying 
this power rule.
    \begin{multicols}{2}
    \begin{enumerate}
    \item \spacer$f(x) = x^5$
    \item \spacer$f(x) = 3x^2$
    \item \spacer$f(x) = -5x^4$
    \item \spacer$f(x) = -7x^{10}$
    \item \spacer$f(x) = \frac{x^3}{18}$
    \item \spacer$f(x) = \frac{2x^6}{9}$
    \item \spacer$f(x) = x^{-2}$
    \item \spacer$f(x) = -2x^{-4}$
    \item \spacer$f(x) = \frac{1}{x^3}$
    \item \spacer$f(x) = \frac{5}{4x^4}$
    \end{enumerate}
    \end{multicols}

\item For each of the following functions find their derivatives.
    \begin{multicols}{2}
    \begin{enumerate}
    \item \sspacer$f(x) = e^x$
    \item \sspacer$f(x) = e^{2x}$
    \item \sspacer$f(x) = e^{-x}$
    \item \sspacer$f(x) = -e^{\frac{x}{2}}$
    \item \sspacer$f(x) = 2^x$
    \item \sspacer$f(x) = 3^{8x}$
    \item \sspacer$f(x) = 2^{-10x}$
    \item \sspacer$f(x) = -5^{-\frac{x}{2}}$
    \end{enumerate}
    \end{multicols}

\item For each of the following functions find their derivatives.
    \begin{multicols}{2}
    \begin{enumerate}
    \item \rule[-0.5em]{0em}{1.5em}$f(x) = \ln(x)$
    \item \rule[-0.5em]{0em}{1.5em}$f(x) = 4\ln(x)$
    \item \rule[-0.5em]{0em}{1.5em}$f(x) = -2\ln(x)$
    \item \rule[-0.5em]{0em}{1.5em}$f(x) = 2\ln(2x)$
    \item \rule[-0.5em]{0em}{1.5em}$f(x) = \log_2(x)$
    \item \rule[-0.5em]{0em}{1.5em}$f(x) = -\log_{10}(x)$
    \item \rule[-0.5em]{0em}{1.5em}$f(x) = \log_3(2x)$
    \item \rule[-0.5em]{0em}{1.5em}$f(x) = 2\log_2(4x)$
    \end{enumerate}
    \end{multicols}

\item For each of the following functions find their derivatives.
    \begin{multicols}{2}
    \begin{enumerate}
    \item \sspacer$f(x) = \sin(x)$
    \item \sspacer$f(x) = \cos(x)$
    \item \sspacer$f(x) = \tan(x)$
    \item \sspacer$f(x) = \sin(3x)$
    \item \sspacer$f(x) = -2\cos(4x)$
    \item \sspacer$f(x) = 3\tan(x)$
    \end{enumerate}
    \end{multicols}

\item For each of the following functions find their derivatives.
    \begin{multicols}{2}
    \begin{enumerate}
    \item \sspacer$f(x) = \sin^{-1}(x)$
    \item \sspacer$f(x) = -\cos^{-1}(x)$
    \item \sspacer$f(x) = \tan^{-1}(x)$
    \item \sspacer$f(x) = 2\sin^{-1}(2x)$
    \item \sspacer$f(x) = 15\cos^{-1}\left(\frac{x}{5}\right)$
    \item \sspacer$f(x) = 3\tan^{-1}\left(\frac{x}{5}\right)$
    \end{enumerate}
    \end{multicols}

\end{enumerate}
\newpage
\subsection*{Answers}

\begin{enumerate}
\item
    \begin{multicols}{2}
    \begin{enumerate}
    \item \sspacer$f'(x) = 3x^2$
    \item \sspacer$f'(x) = 4$
    \item \sspacer$f'(x) = 4x - 3$
    \item \sspacer$f'(x) = 4x + 1$
    \item \sspacer$f'(x) = 3x^2 - 8x + 2$
    \item \sspacer$f'(x) = -\frac{2}{x^2}$
    \end{enumerate}
    \end{multicols}

\item
    \begin{multicols}{2}
    \begin{enumerate}
    \item \spacer$f'(x) = 5x^4$
    \item \spacer$f'(x) = 6x$
    \item \spacer$f'(x) = -20x^3$
    \item \spacer$f'(x) = -70x^9$
    \item \spacer$f'(x) = \frac{x^2}{6}$
    \item \spacer$f'(x) = \frac{4x^5}{3}$
    \item \spacer$f'(x) = -2x^{-3}$ or $\frac{-2}{x^3}$
    \item \spacer$f'(x) = 8x^{-5}$ or $\frac{8}{x^5}$
    \item \spacer$f'(x) = \frac{-3}{x^4}$
    \item \spacer$f'(x) = \frac{-5}{x^5}$
    \item \spacer$f'(x) = 30x^4 + 12x^3$ or $6x^3(5x + 2)$
    \end{enumerate}
    \end{multicols}

\item
    \begin{multicols}{2}
    \begin{enumerate}
    \item \spacer$f'(x) = e^x$
    \item \spacer$f'(x) = 2e^{2x}$
    \item \spacer$f'(x) = -e^{-x}$
    \item \spacer$f'(x) = -\frac{e^{\frac{x}{2}}}{2}$
    \item \spacer$f'(x) = \ln(2)2^x$
    \item \spacer$f'(x) = 8\ln(3)3^{8x}$
    \item \spacer$f'(x) = -10\ln(2)2^{-10x}$
    \item \spacer$f'(x) = \frac{\ln(5)5^{-\frac{x}{2}}}{2}$
    \end{enumerate}
    \end{multicols}

\item
    \begin{multicols}{2}
    \begin{enumerate}
    \item \spacer$f'(x) = \frac{1}{x}$
    \item \spacer$f'(x) = \frac{4}{x}$
    \item \spacer$f'(x) = -\frac{2}{x}$
    \item \spacer$f'(x) = \frac{4}{2x}$
    \item \spacer$f'(x) = \frac{1}{\ln(2)x}$
    \item \spacer$f'(x) = -\frac{1}{\ln(10)x}$
    \item \spacer$f'(x) = \frac{2}{2\ln(3)x}$
    \item \spacer$f'(x) = \frac{8}{4\ln(2)x}$
    \end{enumerate}
    \end{multicols}

\newpage
\item
    \begin{multicols}{2}
    \begin{enumerate}
    \item \sspacer$f'(x) = \cos(x)$
    \item \sspacer$f'(x) = -\sin(x)$
    \item \sspacer$f'(x) = \sec^2(x)$
    \item \sspacer$f'(x) = 3\cos(3x)$
    \item \sspacer$f'(x) = 8\sin(4x)$
    \item \sspacer$f'(x) = 3\sec^2(x)$
    \end{enumerate}
    \end{multicols}

\item
    \begin{multicols}{2}
    \begin{enumerate}
    \item \spacer$f'(x) = \frac{1}{\sqrt{1-x^2}}$
    \item \spacer$f'(x) = \frac{1}{\sqrt{1-x^2}}$
    \item \spacer$f'(x) = \frac{1}{1+x^2}$
    \item \spacer$f'(x) = \frac{3}{\sqrt{1-4x^2}}$
    \item \spacer$f'(x) = \frac{3}{\sqrt{1-\frac{x^2}{25}}}$
    \item \spacer$f'(x) = \frac{15}{25 + x^2}$
    \end{enumerate}
    \end{multicols}

\end{enumerate}

\end{document}
