\documentclass[a4paper,12pt]{article}

\usepackage{worksheet}

\newcommand{\deriv}[3][]{\frac{d^{#1}#2}{d#3^{#1}}}

\begin{document}

\section*{Finding Derivatives Expanded}

\subsection*{Question Bank}

\begin{enumerate}
\item For the following functions, find their derivatives by first 
rearranging to a suitable form then by applying the power rule.
    \begin{multicols}{2}
    \begin{enumerate}
    \item \spacer$f(x) = 3x^2(2x^3 + x^2)$
    \item \spacer$f(x) = 4x^3\left(x^2 - 2x + \frac{3}{2}\right)$
    \item \spacer$f(x) = x^{\frac{1}{2}}$
    \item \spacer$f(x) = \frac{3}{4}x^{\frac{2}{3}}$
    \item \spacer$f(x) = x^{-\frac{1}{2}}$
    \item \spacer$f(x) = 5\sqrt{x}$
    \item \spacer$f(x) = 4\sqrt{x^3}$
    \item \spacer$f(x) = \frac{8}{3}x\sqrt{x}$
    \item \spacer$f(x) = \frac{2}{\sqrt{x}}$
    \item \spacer$f(x) = \frac{5}{\sqrt[3]{x^2}}$
    \end{enumerate}
    \end{multicols}

\item For each of the following functions find their derivatives.
    \begin{multicols}{2}
    \begin{enumerate}
    \item \spacer$f(x) = (4x^3 - 4x)^4$
    \item \spacer$f(x) = 2(6x^2 - 3x + 5)^3$
    \item \spacer$f(x) = \left(\frac{x^3}{3} + 4x^2\right)^4$
    \item \spacer$f(x) = -5\left(\frac{x^4 - 5x^3}{4}\right)^6$
    \item \spacer$f(x) = -\frac{2}{3x^2 - 5}$
    \item \spacer$f(x) = \frac{1}{2(3x^4 + 2x^2)^2}$
    \end{enumerate}
    \end{multicols}

\item For each of the following functions find their derivatives.
    \begin{multicols}{2}
    \begin{enumerate}
    \item \spacer$f(x) = (e^x)^3$
    \item \spacer$f(x) = (e^x + 4)^4$
    \item \spacer$f(x) = \frac{2}{(e^x)^2}$
    \item \spacer$f(x) = -\frac{2}{e^x}$
    \item \spacer$f(x) = 2(-e^x)^3$
    \item \spacer$f(x) = \sqrt{e^x}$
    \item \spacer$f(x) = 5\sqrt[3]{e^x}$
    \item \spacer$f(x) = \frac{4}{\sqrt{(e^x)^3}}$
    \end{enumerate}
    \end{multicols}

\newpage
\item For each of the following functions find their derivatives. 
    \begin{multicols}{2}
    \begin{enumerate}
    \item \sspacer$f(x) = e^{(x^2)}$
    \item \sspacer$f(x) = e^{(x^3)}$
    \item \sspacer$f(x) = 2^{(3x^2)}$
    \item \sspacer$f(x) = 3^{\left(\frac{1}{x}\right)}$
    \item \sspacer$f(x) = e^{\left(-\frac{1}{x^2}\right)}$
    \item \sspacer$f(x) = e^{(x^3 - 3x^2)}$
    \item \sspacer$f(x) = 10^{\sqrt{x}}$
    \item \sspacer$f(x) = 2^{\sqrt{x^3}}$
    \end{enumerate}
    \end{multicols}

\item For each of the following functions find their derivatives.
    \begin{multicols}{2}
    \begin{enumerate}
    \item \sspacer$f(x) = (x^2 + 3)e^x$
    \item \sspacer$f(x) = (2x^3 + 4x^2)e^x$
    \item \sspacer$f(x) = 10x^2(1 - e^{-3x})$
    \item \sspacer$f(x) = (e^{(3x^2)} + 4x)(x^2 - 2x)$
    \item \sspacer$f(x) = (x^2 + 2)^3e^x$
    \item \sspacer$f(x) = (9x^3 + 2x)^4e^{3x}$
    \end{enumerate}
    \end{multicols}

\item For each of the following functions find their derivatives.
    \begin{multicols}{2}
    \begin{enumerate}
    \item \spacer$f(x) = \ln(3x^2)$
    \item \spacer$f(x) = \ln(x^3 + 4x^2)$
    \item \spacer$f(x) = \ln\left(4x^3 + \frac{2}{x}\right)$
    \item \spacer$f(x) = \ln\left(\frac{3}{4x^4 + 2x^2}\right)$
    \item \spacer$f(x) = 3(\ln(x))^3$
    \item \spacer$f(x) = -17(\ln(x))^7$
    \item \spacer$f(x) = (\ln(2x^3 + 3))^8$
    \item \spacer$f(x) = 4(\ln(4x^2 - 8))^4$
    \end{enumerate}
    \end{multicols}

\item For each of the following functions find their derivatives.
    \begin{multicols}{2}
    \begin{enumerate}
    \item \sspacer$f(x) = (4x^9 + 8x^5 + 2)\ln(x)$
    \item \sspacer$f(x) = (7x^4 + 2x^2)\ln(2x)$
    \item \sspacer$f(x) = (x + 4)^4\ln(4x)$
    \item \sspacer$f(x) = (x^2 + 3x - 28)\ln(x-4)$
    \item \sspacer$f(x) = (3x + 5)^4\ln(3x+5)$
    \item \sspacer$f(x) = (5x^4 + 3x)^3\ln(5x^4 + 3x)$
    \end{enumerate}
    \end{multicols}

%\item For each of the following functions find their derivatives.
%    \begin{multicols}{2}
%    \begin{enumerate}
%    \item 
%    \end{enumerate}
%    \end{multicols}
\end{enumerate}
\newpage
\subsection*{Answers}

\begin{enumerate}
\item
    \begin{multicols}{2}
    \begin{enumerate}
    \item \spacer$f'(x) = 30x^4 + 12x^3$ or $6x^3(5x + 2)$
    \item \spacer$f'(x) = 20x^4 - 8x^3 + 18x^2$ or $2x^2(10x^2 - 4x + 9)$
    \item \spacer$f'(x) = \frac{1}{2}x^{-\frac{1}{2}}$ or $\frac{1}{2\sqrt{x}}$
    \item \spacer$f'(x) = \frac{1}{2}x^{-\frac{1}{3}}$ or $\frac{1}{2\sqrt[3]{x}}$
    \item \spacer$f'(x) = -\frac{1}{2}x^{-\frac{3}{2}}$ or $-\frac{1}{2\sqrt{x^3}}$
    \item \spacer$f'(x) = \frac{5}{2\sqrt{x}}$
    \item \spacer$f'(x) = 6\sqrt{x}$
    \item \spacer$f'(x) = 4\sqrt{x}$
    \item \spacer$f'(x) = -\frac{1}{\sqrt{x^3}}$
    \item \spacer$f'(x) = -\frac{10}{3\sqrt[3]{x^5}}$
    \end{enumerate}
    \end{multicols}

\item
    \begin{enumerate}
    \item \spacer$f'(x) = 16(3x^2 - 1)(4x^3 - 4x)^3$
    \item \spacer$f'(x) = 18(4x - 1)(6x^2 - 3x + 5)^2$
    \item \spacer$f'(x) = 4(x^2 + 8x)\left(\frac{x^3}{3} + 4x^2\right)^3$
    \item \spacer$f'(x) = -\frac{15}{2}(4x^3 - 15x^2)\left(\frac{x^4 - 5x^3}{4}\right)^5$
    \item \spacer$f'(x) = \frac{12x}{(3x^2 - 5)^2}$
    \item \spacer$f'(x) = -\frac{4x(3x^2 + 1)}{(3x^4 + 2x^2)^3}$
    \end{enumerate}

\item
    \begin{multicols}{2}
    \begin{enumerate}
    \item \spacer$f'(x) = 3e^{3x}$
    \item \spacer$f'(x) = 4e^x(e^x + 4)^3$
    \item \spacer$f'(x) = -\frac{4}{e^{2x}}$ or $-4e^{-2x}$
    \item \spacer$f'(x) = 2e^{-x}$
    \item \spacer$f'(x) = 6(-e^x)^3$
    \item \spacer$f'(x) = \frac{1}{2}e^{\frac{x}{2}}$
    \item \spacer$f'(x) = \frac{5}{3}e^{\frac{x}{3}}$
    \item \spacer$f'(x) = 6e^{\frac{3x}{2}}$
    \end{enumerate}
    \end{multicols}

\item
    \begin{multicols}{2}
    \begin{enumerate}
    \item \spacer$f'(x) = 2xe^{(x^2)}$
    \item \spacer$f'(x) = 3x^2e^{(x^3)}$
    \item \spacer$f'(x) = 3\ln(2)x2^{(3x^2)}$
    \item \spacer$f'(x) = -\frac{\ln(3)}{x^2}3^{(\frac{1}{x})}$
    \item \spacer$f'(x) = \frac{2}{x^3}e^{(-\frac{1}{x^2})}$
    \item \spacer$f'(x) = (3x^2 - 6x)e^{(x^3 - 3x^2)}$
    \item \spacer$f'(x) = \frac{\ln(10)}{2\sqrt{x}}10^{\sqrt{x}}$
    \item \spacer$f'(x) = \frac{3\ln(2)\sqrt{x}}{2}2^{\sqrt{x^3}}$
    \end{enumerate}
    \end{multicols}

\item
    \begin{enumerate}
    \item \sspacer$f'(x) = (x^2 + 2x + 3)e^x$
    \item \sspacer$f'(x) = 2(x^3 + 5x^2 + 4x)e^x$
    \item \sspacer$f'(x) = 10x(2 + (3x - 2)e^{-3x})$
    \item \sspacer$f'(x) = x(13x - 24)e^{(3x^2)} + 4(x^3 - 2x^2 + 2x - 2)$
    \item \sspacer$f'(x) = (x^2+2)^2(x^2 + x + 2)e^x$
    \item \sspacer$f'(x) = (9x^3 + 2x)^3(27x^3 + 108x^2 + 6x + 8)e^{3x}$
    \end{enumerate}

\item
    \begin{multicols}{2}
    \begin{enumerate}
    \item \spacer$f'(x) = \frac{6}{3x}$
    \item \spacer$f'(x) = \frac{3x + 8}{x^2 + 4x}$
    \item \spacer$f'(x) = \frac{6x^4 + 1}{4x^5 + 2x}$
    \item \spacer$f'(x) = -\frac{16x^2 + 4}{4x^3 + 2x}$
    \item \spacer$f'(x) =\frac{12}{x}(\ln(x))^3$
    \item \spacer$f'(x) = -\frac{119}{x}(\ln(x))^6$
    \item \spacer$f'(x) = \frac{48x^2}{2x^3 + 3}(\ln(2x^3 + 3))^7$
    \item \spacer$f'(x) = \frac{32x}{x^2-2}(\ln(4x^2 - 8))^3$
    \end{enumerate}
    \end{multicols}

\item
    \begin{enumerate}
    \item \sspacer$f'(x) = 4(9x^8 + 10x^4)\ln(x) + \frac{2(2x^9 + 4x^5 + 1)}{x}$
    \item \sspacer$f'(x) = 4(7x^3 + x)\ln(2x) + x(7x^2 + 2)$
    \item \sspacer$f'(x) = (x+4)^3\left(4\ln(4x) + 1 + \frac{4}{x}\right)$
    \item \sspacer$f'(x) = (2x+3)\ln(x-4) + x + 7$
    \item \sspacer$f'(x) = 3(3x+5)^3(4\ln(3x+5) + 1)$
    \item \sspacer$f'(x) = (20x^3 + 3)(5x^4 + 3x)^2(3\ln(5x^4 + 3x) + 1)$
    \end{enumerate}

%\item
%    \begin{multicols}{2}
%    \begin{enumerate}
%    \item
%    \end{enumerate}
%    \end{multicols}

\end{enumerate}

\end{document}
