\documentclass[a4paper,12pt]{article}

\usepackage{worksheet}

\begin{document}

\large
\section*{Gradient Intercept and General Form Conversion}

\subsection*{Question Bank}

\textsc{Note}: For answers that are fractions, leave them as 
fractions but simplify them if possible.

\begin{enumerate}
\item Equations of the form $y = mx + c$ are in gradient-intercept
form. So called, because $m$ (the coefficient of $x$) tells you 
the gradient of the line and $c$ tells you the $y$-intercept of 
the line. As a warm up, for each of the following equations 
determine i) their gradient, and ii) their $y$-intercept.
    \begin{multicols}{2}
    \begin{enumerate}
    \item $y = 2x + 5$
    \item $y = 3x - 2$
    \item $y = -x + 3$
    \item $y = -3x + 13$
    \item $y = 155x + 240$
    \item $y = \frac{1}{3}x - 3$
    \item $y = \frac{x}{2} + 23$
    \item $y = -\frac{3}{7}x - \frac{4}{9}$
    \item $y = -\frac{2x}{5} + \frac{6}{5}$
    \end{enumerate}
    \end{multicols}

\item An often under-stressed feature of the gradient-intercept
form is that \textbf{$y$ must have a coefficient of 1}, hence an equation
such as $3y = 6x - 5$ is not in gradient-intercept from and we 
\textbf{cannot} say $6$ is the gradient and $-5$ is the $y$-intercept.
We must divide both sides by the current coefficient of $y$ (3)
to make $y$'s coefficient 1,
\begin{align*}
    \frac{3y}{3} &= \frac{6x - 5}{3}, \\
    y &= \frac{6x}{3} - \frac{5}{3}, \\
    y &= 2x - \frac{5}{3}.
\end{align*}
For each of the following equations, i) convert them into 
gradient-intercept form, ii) determine their gradient and 
iii) determine their $y$-intercept.
    \begin{multicols}{2}
    \begin{enumerate}
    % simplify nice
    \item $2y = 4x - 6$
    \item $3y = -6x + 12$
    \item $-5y = 5x + 25$
    \item $-7y = -21x - 28$
    % one term remains a fraction
    \item $2y = 5x + 6$
    \item $-5y = 15x - 17$
    \item $-6y = -15x + 42$
    \item $3y = -9x + 13$
    % both terms remain fractions
    \item $-3y = -5x - 8$
    \item $8y = 12x - 4$
    \item $4y = 3x + 18$
    \item $-9y = 21x + 39$.
    % fraction on LHS
    \item $\frac{y}{2} = 2x - \frac{1}{2}$
    \item $\frac{y}{3} = -\frac{4}{3}x + 12$
    \item $-\frac{y}{5} = 2x - 8$
    \item $-\frac{y}{2} = -\frac{3x}{2} - \frac{7}{6}$
    \item $\frac{3y}{2} = 6x + 15$
    \item $\frac{5y}{3} = -x - 15$
    \item $-\frac{2y}{7} = \frac{3x}{14} + 4$
    \item $-\frac{9}{4}y = -\frac{27}{2}x + \frac{7}{4}$
    \end{enumerate}
    \end{multicols}

\item The general form of an equation is $ax + by + c = 0$.
In this form $c$ \textbf{is not the same} as the $c$ in the 
gradient-intercept form, and \textbf{does not} represent the
$y$-intercept. Since this form does not tell us much information
we usually convert from general form into gradient-intercept 
form if we plan to draw the line. To do this first we need
to isolate $y$, consider the equation
$$4x - 2y - 5 = 0,$$
first we can subtract $4x$ from then add $5$ to both
sides,
\begin{align*}
4x - 2y - 5 &= 0, \\
4x - 2y - 5 - 4x &= 0 - 4x, \\
-2y - 5 &= -4x, \\
-2y - 5 + 5 &= -4x + 5, \\
-2y &= -4x + 5.
\end{align*}
Then we can divide both sides by $-2$,
\begin{align*}
\frac{-2y}{-2} &= \frac{-4x + 5}{-2}, \\
y &= \frac{-4x}{-2} + \frac{5}{-2}, \\
y &= 2x - \frac{5}{2}.
\end{align*}
For each of the following general form equations, rearrange 
them into gradient-intercept from.
    \begin{multicols}{2}
    \begin{enumerate}
    \item $x + y - 4 = 0$
    \item $2x - y + 3 = 0$
    \item $x + 2y + 6 = 0$
    \item $2x - 3y - 7 = 0$
    \item $-5x - 3y = 0$
    \item $6x + 9y + 24 = 0$
    \item $-x + 2y - 12 = 0$
    \item $12x - 8y + 14 = 0$
    \item $2x + \frac{3}{4}y + 6 = 0$
    \item $-7x - \frac{14}{3}y - \frac{7}{2} = 0$
    \item $-\frac{2}{5}x - 3y + 4 = 0$
    \item $\frac{3}{13}x + 12y + \frac{9}{26} = 0$
    \item $\frac{12}{5}x - \frac{1}{7}y + 2 = 0$
    \item $-\frac{8}{21}x + \frac{42}{25}y - \frac{2}{7} = 0$
    \end{enumerate}
    \end{multicols}

\item To convert from gradient-intercept form into genera
form, we need to ``move'' all the terms onto one side so
that one side of the equation is 0. Consider the equation 
$$y = -3x + \frac{3}{4},$$
we would add $3x$ to, then subtract $\frac{3}{4}$ from, 
both sides of the equation,
\begin{align*}
y + 3x &= -3x + \frac{3}{4} + 3x, \\
y + 3x &= \frac{3}{4}, \\
y + 3x - \frac{3}{4} &= \frac{3}{4} - \frac{3}{4}, \\
y + 3x - \frac{3}{4} &= 0.
\end{align*}
Then to make the equation look nicer, we might move the terms
such that it looks more like the form $ax + by + c = 0$,
$$3x + y - \frac{3}{4} = 0.$$
An optional extra that is often nice, is to remove fractions 
from the equation. Since ours has $\frac{3}{4}$ we might 
multiply both sides by 4
\begin{align*}
4\left(3x + y - \frac{3}{4}\right) &= 0\times 4, \\
(4 \times 3x) + (4 \times y) + \left(4 \times -\frac{3}{4}\right) &= 0, \\
12x + 4y - 3 = 0.
\end{align*}
For each of the following equations in gradient-intercept form, 
convert them into general form and simplify where possible.
\emph{(Your answers to these questions might not exactly match the 
provided solutions because there are many valid general forms
for each line, if this happens try to multiply or divide your
answer and see if you can match the provided solution. The 
solutions tend to have no fractions and a positive coefficient of
$x$)}
    \begin{multicols}{2}
    \begin{enumerate}
    \item $y = x - 4$
    \item $y = -2x + 5$
    \item $y = -3x - 2$
    \item $y = 2x + 4$
    \item $y = 7x - 10$
    \item $y = 5x + 20$
    \item $y = \frac{1}{3}x + 5$
    \item $y = -\frac{1}{7}x + 2$
    \item $y = -7x + \frac{49}{6}$
    \item $y = 4x - \frac{9}{10}$
    \item $y = \frac{12}{5}x - \frac{10}{3}$
    \item $y = -\frac{4}{5}x - \frac{3}{4}$
    \item $y = -\frac{3}{4}x + \frac{7}{2}$
    \item $y = \frac{5}{12}x - \frac{5}{18}$
    \end{enumerate}
    \end{multicols}

\end{enumerate}

\newpage
\subsection*{Answers}

\begin{enumerate}
\item
    \begin{multicols}{2}
    \begin{enumerate}
    \item
        \begin{enumerate}
        \item $2$
        \item $5$
        \end{enumerate}
    \item
        \begin{enumerate}
        \item $3$
        \item $-2$
        \end{enumerate}
    \item
        \begin{enumerate}
        \item $-1$
        \item $3$
        \end{enumerate}
    \item
        \begin{enumerate}
        \item $-3$
        \item $13$
        \end{enumerate}
    \item
        \begin{enumerate}
        \item $155$
        \item $240$
        \end{enumerate}
    \item
        \begin{enumerate}
        \item $\frac{1}{3}$
        \item $-3$
        \end{enumerate}
    \item
        \begin{enumerate}
        \item $\frac{1}{2}$
        \item $23$
        \end{enumerate}
    \item
        \begin{enumerate}
        \item $-\frac{3}{7}$
        \item $-\frac{4}{9}$
        \end{enumerate}
    \item
        \begin{enumerate}
        \item $-\frac{2}{5}$
        \item $\frac{6}{5}$
        \end{enumerate}
    \end{enumerate}
    \end{multicols}

\item
    \begin{multicols}{2}
    \begin{enumerate}
    \item
        \begin{enumerate}
        \item $y = 2x - 3$
        \item $2$
        \item $-3$
        \end{enumerate}
    \item
        \begin{enumerate}
        \item $y = -2x + 4$
        \item $-2$
        \item $4$
        \end{enumerate}
    \item
        \begin{enumerate}
        \item $y = -x - 5$
        \item $-1$
        \item $-5$
        \end{enumerate}
    \item
        \begin{enumerate}
        \item $y = 3x + 4$
        \item $3$
        \item $4$
        \end{enumerate}
    \item
        \begin{enumerate}
        \item $y = \frac{5}{2}x + 3$
        \item $\frac{5}{2}$
        \item $3$
        \end{enumerate}
    \item
        \begin{enumerate}
        \item $y = -3x + \frac{17}{5}$
        \item $-3$
        \item $\frac{17}{5}$
        \end{enumerate}
    \item
        \begin{enumerate}
        \item $y = \frac{5}{2}x - 7$
        \item $\frac{5}{2}$
        \item $-7$
        \end{enumerate}
    \item
        \begin{enumerate}
        \item $y = -3x + \frac{13}{3}$
        \item $-3$
        \item $\frac{13}{3}$
        \end{enumerate}
    \item
        \begin{enumerate}
        \item $y = \frac{5}{3}x + \frac{8}{3}$
        \item $\frac{5}{3}$
        \item $\frac{8}{3}$
        \end{enumerate}
    \item
        \begin{enumerate}
        \item $y = \frac{3}{2}x - \frac{1}{2}$
        \item $\frac{3}{2}$
        \item $-\frac{1}{2}$
        \end{enumerate}
    \item
        \begin{enumerate}
        \item $y = \frac{3}{4}x + \frac{9}{2}$
        \item $\frac{3}{4}$
        \item $\frac{9}{2}$
        \end{enumerate}
    \item
        \begin{enumerate}
        \item $y = -\frac{7}{3}x - \frac{13}{3}$
        \item $-\frac{7}{3}$
        \item $-\frac{13}{3}$
        \end{enumerate}
    \item
        \begin{enumerate}
        \item $y = 4x - 1$
        \item $4$
        \item $-1$
        \end{enumerate}
    \item
        \begin{enumerate}
        \item $y = -4x + 36$
        \item $-4$
        \item $36$
        \end{enumerate}
    \item
        \begin{enumerate}
        \item $y = -10x + 40$
        \item $-10$
        \item $40$
        \end{enumerate}
    \item
        \begin{enumerate}
        \item $y = 3x + \frac{7}{3}$
        \item $3$
        \item $\frac{7}{3}$
        \end{enumerate}
    \item
        \begin{enumerate}
        \item $y = 4x + 10$
        \item $4$
        \item $10$
        \end{enumerate}
    \item
        \begin{enumerate}
        \item $y = -\frac{3}{5}x - 9$
        \item $-\frac{3}{5}$
        \item $-9$
        \end{enumerate}
    \item
        \begin{enumerate}
        \item $y = -\frac{3}{4}x - 14$
        \item $-\frac{3}{4}$
        \item $-14$
        \end{enumerate}
    \item
        \begin{enumerate}
        \item $y = 6x - \frac{7}{9}$
        \item $6$
        \item $-\frac{7}{9}$
        \end{enumerate}
    \end{enumerate}
    \end{multicols}

\item
    \begin{multicols}{2}
    \begin{enumerate}
    \item $y = -x + 4$
    \item $y = 2x + 3$
    \item $y = -\frac{1}{2}x - 3$
    \item $y = \frac{2}{3}x - \frac{7}{3}$
    \item $y = -\frac{5}{3}x$
    \item $y = -\frac{2}{3}x - \frac{8}{3}$
    \item $y = \frac{1}{2}x + 6$
    \item $y = \frac{3}{2}x + \frac{7}{4}$
    \item $y = -\frac{8}{3}x - 8$
    \item $y = -\frac{3}{2}x - \frac{3}{4}$
    \item $y = -\frac{2}{15}x + \frac{4}{3}$
    \item $y = -\frac{1}{52}x - \frac{3}{104}$
    \item $y = \frac{84}{5}x + 14$
    \item $y = \frac{100}{441}x + \frac{25}{147}$
    \end{enumerate}
    \end{multicols}

\item
    \begin{multicols}{2}
    \begin{enumerate}
    \item $x - y - 4 = 0$
    \item $2x + y - 5 = 0$
    \item $3x + y + 2 = 0$
    \item $2x - y + 4 = 0$
    \item $7x - y - 10 = 0$
    \item $5x - y + 20 = 0$
    \item $x - 3y + 15 = 0$
    \item $x + 7y - 14 = 0$
    \item $42x + 6y - 49 = 0$
    \item $40x - 10y - 9 = 0$
    \item $36x - 15y - 50 = 0$
    \item $16x + 20y + 15 = 0$
    \item $3x + 4y - 14 = 0$
    \item $15x - 36y - 10 = 0 $
    \end{enumerate}
    \end{multicols}

\end{enumerate}

\end{document}
